src/certigrad/aevb/aevb_correct.lean
@@ -1,0 +1,37 @@
+/-
+Copyright (c) 2017 Daniel Selsam. All rights reserved.
+Released under Apache 2.0 license as described in the file LICENSE.
+Author: Daniel Selsam
+
+Proofs that integrating out the KL and reparametizing are sound when
+applied to the naive variational encoder.
+-/
+import .util .graph .prog .grads_correct .transformations ..prove_model_ok ..pre ..backprop_correct
+
+set_option profiler true
+
+namespace certigrad
+namespace aevb
+
+open graph list tactic certigrad.tactic
+
+theorem aevb_backprop_correct (a : arch) (ws : weights a) (x_data : T [a^.n_in, a^.n_x]) :
+let g₀ : graph := naive_aevb a x_data in
+let g_aevb : graph := reparam (integrate_kl g₀) in
+let fdict : env := mk_input_dict ws g₀ in
+∀ (tgt : reference) (idx : ℕ) (H_at_idx : at_idx g₀^.targets idx tgt),
+∇ (λ θ₀, E (graph.to_dist (λ m, ⟦sum_costs m g₀^.costs⟧) (env.insert tgt θ₀ fdict) g₀^.nodes) dvec.head) (env.get tgt fdict)
+=
+E (graph.to_dist (λ m, backprop g_aevb^.costs g_aevb^.nodes m g_aevb^.targets) fdict g_aevb^.nodes) (λ dict, dvec.get tgt.2 dict idx) :=
+begin
+whnf_target,
+intros tgt idx H_at_idx,
+simp only [@aevb_transformations_sound a ws x_data tgt idx H_at_idx],
+apply final_backprop_correct,
+rw [naive_aevb_as_graph] at H_at_idx,
+rw [naive_aevb_as_graph],
+exact H_at_idx
+end
+
+end aevb
+end certigrad
