src/certigrad/aevb/grads_correct.lean
@@ -6,7 +6,7 @@ Author: Daniel Selsam
 Proofs that integrating out the KL and reparametizing are sound when
 applied to the naive variational encoder.
 -/
-import .util .graph .prog ..prove_model_ok ..pre ..backprop_correct
+import .util .graph ..prove_model_ok ..pre ..backprop_correct
 
 set_option profiler true
 
@@ -15,8 +15,8 @@ namespace aevb
 
 open graph list tactic certigrad.tactic
 
-theorem aevb_backprop_correct (a : arch) (ws : weights a) (x_data : T [a^.n_in, a^.n_x]) :
-let g : graph := reparam (integrate_kl $ graph_naive a x_data in
+theorem final_backprop_correct (a : arch) (ws : weights a) (x_data : T [a^.n_in, a^.n_x]) :
+let g : graph := reparam (integrate_kl $ naive_aevb a x_data) in
 let fdict : env := mk_input_dict ws g in
 ∀ (tgt : reference) (idx : ℕ) (H_at_idx : at_idx g^.targets idx tgt),
 ∇ (λ θ₀, E (graph.to_dist (λ m, ⟦sum_costs m g^.costs⟧) (env.insert tgt θ₀ fdict) g^.nodes) dvec.head) (env.get tgt fdict)
