src/certigrad/aevb/transformations.lean
@@ -6,7 +6,7 @@ Author: Daniel Selsam
 Proofs that integrating out the KL and reparametizing are sound when
 applied to the naive variational encoder.
 -/
-import .util .naive ..prove_model_ok
+import .util .prog .graph ..prove_model_ok ..kl
 
 namespace certigrad
 namespace aevb
@@ -14,37 +14,49 @@ namespace aevb
 open graph list tactic certigrad.tactic
 
 lemma integrate_kl_sound (a : arch) (ws : weights a) (x_data : T [a^.n_in, a^.n_x]) :
-let g : graph   := graph_naive a x_data, fdict : env := mk_input_dict ws g in
-E (graph.to_dist (λ m, ⟦sum_costs m (integrate_kl g)^.costs⟧) fdict (integrate_kl g)^.nodes) dvec.head
+let g₀ : graph := graph_naive a x_data, fdict : env := mk_input_dict ws g₀ in
+∀ (tgt : reference) (idx : ℕ) (H_at_idx : at_idx g₀^.targets idx tgt) (θ : T tgt.2),
+E (graph.to_dist (λ m, ⟦sum_costs m (integrate_kl g₀)^.costs⟧) (env.insert tgt θ fdict) (integrate_kl g₀)^.nodes) dvec.head
 =
-E (graph.to_dist (λ m, ⟦sum_costs m g^.costs⟧) fdict g^.nodes) dvec.head :=
-begin
-whnf_target,
-apply integrate_mvn_iso_kl_correct (ID.str label.encoding_loss) [ID.str label.decoding_loss] (graph_naive a x_data)^.nodes,
-all_goals { cgsimp >> try prove_is_mvn_integrable >> try T.prove_preconditions }
-end
+E (graph.to_dist (λ m, ⟦sum_costs m g₀^.costs⟧) (env.insert tgt θ fdict) g₀^.nodes) dvec.head := sorry
+/-
+by do whnf_target,
+      [tgt, idx, H_at_idx, θ] ← intros | failed,
+      forall_idxs prove_model_base (do
+         to_expr ```(integrate_mvn_iso_kl_correct (ID.str label.encoding_loss) [ID.str label.decoding_loss] (graph_naive a x_data)^.nodes) >>= apply,
+         all_goals (cgsimp >> try prove_is_mvn_integrable >> try T.prove_preconditions)) idx
+-/
 
 lemma reparam_sound (a : arch) (ws : weights a) (x_data : T [a^.n_in, a^.n_x]) :
-let g : graph   := integrate_kl $ graph_naive a x_data, fdict : env := mk_input_dict ws g in
-E (graph.to_dist (λ m, ⟦sum_costs m (reparam g)^.costs⟧) fdict (reparam g)^.nodes) dvec.head
+let g₁ : graph := integrate_kl (graph_naive a x_data), fdict : env := mk_input_dict ws g₁ in
+∀ (tgt : reference) (idx : ℕ) (H_at_idx : at_idx g₁^.targets idx tgt) (θ : T tgt.2),
+E (graph.to_dist (λ m, ⟦sum_costs m (reparam g₁)^.costs⟧) (env.insert tgt θ fdict) (reparam g₁)^.nodes) dvec.head
 =
-E (graph.to_dist (λ m, ⟦sum_costs m g^.costs⟧) fdict g^.nodes) dvec.head :=
-begin
-whnf_target,
-apply reparameterize_correct _ (integrate_kl $ graph_naive a x_data)^.nodes _ (ID.str label.ε, [a^.nz, a^.bs]),
-all_goals { cgsimp }
-end
+E (graph.to_dist (λ m, ⟦sum_costs m g₁^.costs⟧) (env.insert tgt θ fdict) g₁^.nodes) dvec.head := sorry
+/-
+by do whnf_target,
+      [tgt, idx, H_at_idx, θ] ← intros | failed,
+      forall_idxs prove_model_base (do
+         to_expr ```(reparameterize_correct _ (integrate_kl $ graph_naive a x_data)^.nodes _ (ID.str label.ε, [a^.nz, a^.bs])) >>= apply,
+         all_goals cgsimp) idx
+-/
 
 -- TODO(dhs): this is annoying, rw and simp should whnf the let
-lemma aevb_correct {a : arch} (ws : weights a) (x_data : T [a^.n_in, a^.n_x]) :
-let g : graph := graph_naive a x_data, g_aevb : graph := reparam (integrate_kl g), fdict : env := mk_input_dict ws g in
-E (graph.to_dist (λ m, ⟦sum_costs m g_aevb^.costs⟧) fdict g_aevb^.nodes) dvec.head
+lemma aevb_transformations_sound {a : arch} (ws : weights a) (x_data : T [a^.n_in, a^.n_x]) :
+let g₀ : graph := naive_aevb a x_data, g_aevb : graph := reparam (integrate_kl g₀), fdict : env := mk_input_dict ws g₀ in
+∀ (tgt : reference) (idx : ℕ) (H_at_idx : at_idx g₀^.targets idx tgt) (θ : T tgt.2),
+E (graph.to_dist (λ m, ⟦sum_costs m g₀^.costs⟧) (env.insert tgt θ fdict) g₀^.nodes) dvec.head
 =
-E (graph.to_dist (λ m, ⟦sum_costs m g^.costs⟧) fdict g^.nodes) dvec.head :=
+E (graph.to_dist (λ m, ⟦sum_costs m g_aevb^.costs⟧) (env.insert tgt θ fdict) g_aevb^.nodes) dvec.head :=
 begin
-note H₁ := reparam_sound, note H₂ := integrate_kl_sound,
+whnf_target,
+intros tgt idx H_at_idx θ,
+note H₁ := @reparam_sound a ws x_data tgt idx,
+note H₂ := @integrate_kl_sound a ws x_data tgt idx,
 dsimp at *,
-erw [H₁, H₂]
+simp only [naive_aevb_as_graph] at *,
+erw [H₁, H₂],
+all_goals { assumption }
 end
 
 end aevb
